refactor a bit; update Lifted and add a demo

src/Lifted.v
@@ -1,27 +1,65 @@
 Require Import List.
 Import ListNotations.
 
-Definition function_name := nat.
+Require Import Utopia.
+Require Import Monads.
 
+
+Definition function_name := nat.
 
 Inductive expr :=
 | Arg : expr
 | UpVar : nat -> expr
 | Call : expr -> expr -> expr
-| Constr (tag : nat) (args : list expr)
-| Switch (cases : list (nat * expr)) (target : expr)
+| Constr (c : constr_name) (args : list expr)
+| Elim (ty : type_name) (cases : list expr) (target : expr)
 | Close (f : function_name) (free : list expr)
 .
 
 Definition env := list expr.
 
 Inductive value : expr -> Prop :=
-| VConstr : forall tag l, Forall value l -> value (Constr tag l)
+| VConstr : forall ctor args, Forall value args -> value (Constr ctor args)
 | VClose : forall f free, Forall value free -> value (Close f free).
 
-Axiom subst : forall (arg : expr) (vals : list expr) (e : expr), option expr.
+Section subst.
+Open Scope option_monad.
 
-Axiom call_all : forall (f : expr) (args : list expr), expr.
+Definition subst (arg : expr) (vals : list expr) (e : expr) : option expr :=
+    let fix go e :=
+        let fix go_list es : option (list expr) :=
+            match es with
+            | [] => Some []
+            | e :: es => @cons expr <$> go e <*> go_list es
+            end in
+        match e with
+        | Arg => Some arg
+        | UpVar n => nth_error vals n
+        | Call f a => Call <$> go f <*> go a
+        | Constr c es => Constr c <$> go_list es
+        | Elim ty cases target => Elim ty <$> go_list cases <*> go target
+        | Close f free => Close f <$> go_list free
+        end in
+    go e.
+End subst.
+
+
+Fixpoint unroll_elim' (case : expr)
+                      (ctor : constr_name)
+                      (args : list expr)
+                      (mk_rec : expr -> expr)
+                      (idx : nat) : expr :=
+    match args with
+    | [] => case
+    | arg :: args =>
+            let case := Call case arg in
+            let case := if ctor_arg_is_recursive ctor idx
+                then Call case (mk_rec arg) else case in
+            unroll_elim' case ctor args mk_rec (S idx)
+    end.
+
+Fixpoint unroll_elim case ctor args mk_rec :=
+    unroll_elim' case ctor args mk_rec 0.
 
 
 Inductive step (E : env) : expr -> expr -> Prop :=
@@ -38,18 +76,79 @@ Inductive step (E : env) : expr -> expr -> Prop :=
     value v ->
     step E e2 e2' ->
     step E (Call v e2) (Call v e2')
-| SwitchStep : forall t t' cases, step E t t' -> step E (Switch cases t) (Switch cases t')
-| Switchinate : forall tag args cases case arg_n,
-    nth_error cases tag = Some (arg_n, case) ->
-    length args = arg_n ->
-    step E (Switch cases (Constr tag args)) (call_all case args)
 | ConstrStep : forall tag vs e e' es,
     step E e e' ->
     Forall value vs ->
     step E (Constr tag (vs ++ [e] ++ es)) (Constr tag (vs ++ [e'] ++ es))
+| ElimStep : forall t t' ty cases,
+        step E t t' ->
+        step E (Elim ty cases t) (Elim ty cases t')
+| Eliminate : forall c args ty cases case,
+    nth_error cases (constructor_index c) = Some case ->
+    step E (Elim ty cases (Constr c args))
+        (unroll_elim case c args (fun x => Elim ty cases x))
 | CloseStep : forall f vs e e' es,
     step E e e' ->
     Forall value vs ->
     step E (Close f (vs ++ [e] ++ es)) (Close f (vs ++ [e'] ++ es))
-
 .
+
+
+
+(* Demo *)
+
+Definition add_lam_a :=             0.
+Definition add_lam_b :=             1.
+Definition elim_zero_lam_b :=       2.
+Definition elim_succ_lam_a :=       3.
+Definition elim_succ_lam_IHa :=     4.
+Definition elim_succ_lam_b :=       5.
+
+Definition add_reflect := Close add_lam_a [].
+
+Definition add_env : list expr :=
+    (* add_lam_a *)
+    [ Close add_lam_b [Arg]
+    (* add_lam_b *)
+    ; Call (Elim Tnat [Close elim_zero_lam_b []; Close elim_succ_lam_a []] (UpVar 0)) Arg
+    (* elim_zero_lam_b *)
+    ; Arg
+    (* elim_succ_lam_a *)
+    ; Close elim_succ_lam_IHa []
+    (* elim_succ_lam_IHa *)
+    ; Close elim_succ_lam_b [Arg]
+    (* elim_succ_lam_b *)
+    ; Call (UpVar 0) (Constr CS [Arg])
+    ].
+
+Inductive star (E : env) : expr -> expr -> Prop :=
+| StarNil : forall e, star E e e
+| StarCons : forall e e' e'',
+        step E e e' ->
+        star E e' e'' ->
+        star E e e''.
+
+Fixpoint nat_reflect n : expr :=
+    match n with
+    | 0 => Constr CO []
+    | S n => Constr CS [nat_reflect n]
+    end.
+
+Theorem add_1_2 : { x | star add_env
+        (Call (Call add_reflect (nat_reflect 1)) (nat_reflect 2)) x }.
+eexists.
+
+unfold add_reflect.
+eright. eapply CallL, MakeCall; try solve [repeat econstructor].
+eright. eapply MakeCall; try solve [repeat econstructor].
+eright. eapply CallL, Eliminate; try solve [repeat econstructor].
+  compute [unroll_elim unroll_elim' ctor_arg_is_recursive].
+eright. eapply CallL, CallL, MakeCall; try solve [repeat econstructor].
+eright. eapply CallL, CallR, Eliminate; try solve [repeat econstructor].
+  compute [unroll_elim unroll_elim' ctor_arg_is_recursive].
+eright. eapply CallL, MakeCall; try solve [repeat econstructor].
+eright. eapply MakeCall; try solve [repeat econstructor].
+eright. eapply MakeCall; try solve [repeat econstructor].
+eleft.
+Defined.
+Eval compute in proj1_sig add_1_2.
