src/Untyped.v
@@ -4,65 +4,7 @@ Require Import Arith Omega.
 
 Require Import StructTact.StructTactics.
 
-Inductive type_name :=
-| Tnat
-| Tbool
-| Tlist_nat
-.
-
-Inductive constr_name :=
-| CS
-| CO
-| Ctrue
-| Cfalse
-| Cnil
-| Ccons
-.
-
-Definition constructor_index ctor : nat :=
-    match ctor with
-    | CO => 0
-    | CS => 1
-
-    | Cfalse => 0
-    | Ctrue => 1
-
-    | Cnil => 0
-    | Ccons => 1
-    end.
-
-Definition constructor_arg_n ctor : nat :=
-    match ctor with
-    | CO => 0
-    | CS => 1
-
-    | Cfalse => 0
-    | Ctrue => 0
-
-    | Cnil => 0
-    | Ccons => 2
-    end.
-
-Definition ctor_arg_is_recursive ctor pos : bool :=
-    match ctor, pos with
-    | CS, 0 => true
-    | Ccons, 1 => true
-    | _, _ => false
-    end.
-
-Definition type_constr ty idx : option constr_name :=
-    match ty, idx with
-    | Tnat, 0 => Some CO
-    | Tnat, 1 => Some CS
-
-    | Tbool, 0 => Some Cfalse
-    | Tbool, 1 => Some Ctrue
-
-    | Tlist_nat, 0 => Some Cnil
-    | Tlist_nat, 1 => Some Ccons
-
-    | _, _ => None
-    end.
+Require Import Utopia.
 
 
 Inductive expr :=
@@ -235,6 +177,15 @@ Fixpoint nat_reflect n : expr :=
     | 0 => Constr CO []
     | S n => Constr CS [nat_reflect n]
     end.
+
+Definition add_reflect :=
+    (Lam (*a*) (Lam (*b*)
+        (App (Elim Tnat
+            [ Lam (*b*) (Var 0)
+            ; Lam (*a*) (Lam (*IHa*) (Lam (*b*)
+                (App (Var 1) (Constr CS [Var 0]))))
+            ]
+            (Var 1)) (Var 0)))).
 
 Definition fib_reflect :=
     (Lam (*n*) (App (App (Elim Tnat
