src/Monads.v
@@ -1,0 +1,41 @@
+Require Import List.
+Import ListNotations.
+
+
+Fixpoint map_partial {A B : Type} (f : A -> option B) (l : list A) : option (list B) :=
+  match l with
+  | [] => Some []
+  | a :: l' => match f a, map_partial f l' with
+              | Some b, Some l'' => Some (b :: l'')
+              | _, _ => None
+              end
+  end.
+
+
+
+Definition fmap {M : Type -> Type}
+    (bind : forall A B, M A -> (A -> M B) -> M B)
+    (ret : forall A, A -> M A)
+    {A B : Type} (f : A -> B) (x : M A) : M B :=
+    bind _ _ x (fun x => ret _ (f x)).
+
+Definition seq {M : Type -> Type}
+    (bind : forall A B, M A -> (A -> M B) -> M B)
+    (ret : forall A, A -> M A)
+    {A B : Type} (f : M (A -> B)) (x : M A) : M B :=
+    bind _ _ f (fun f => @fmap _ bind ret _ _ f x).
+
+
+
+Definition bind_option {A B : Type} (m : option A) (k : A -> option B) : option B :=
+    match m with
+    | Some x => k x
+    | None => None
+    end.
+
+Notation "x '>>=' f" := (bind_option x f)
+    (at level 42, left associativity) : option_monad.
+Notation "f <$> x" := (fmap (@bind_option) (@Some) f x)
+    (at level 42, left associativity) : option_monad.
+Notation "f <*> x" := (seq (@bind_option) (@Some) f x)
+    (at level 42, left associativity) : option_monad.
