src/Utopia.v
@@ -1,0 +1,62 @@
+
+Inductive type_name :=
+| Tnat
+| Tbool
+| Tlist_nat
+.
+
+Inductive constr_name :=
+| CS
+| CO
+| Ctrue
+| Cfalse
+| Cnil
+| Ccons
+.
+
+Definition constructor_index ctor : nat :=
+    match ctor with
+    | CO => 0
+    | CS => 1
+
+    | Cfalse => 0
+    | Ctrue => 1
+
+    | Cnil => 0
+    | Ccons => 1
+    end.
+
+Definition constructor_arg_n ctor : nat :=
+    match ctor with
+    | CO => 0
+    | CS => 1
+
+    | Cfalse => 0
+    | Ctrue => 0
+
+    | Cnil => 0
+    | Ccons => 2
+    end.
+
+Definition ctor_arg_is_recursive ctor pos : bool :=
+    match ctor, pos with
+    | CS, 0 => true
+    | Ccons, 1 => true
+    | _, _ => false
+    end.
+
+Definition type_constr ty idx : option constr_name :=
+    match ty, idx with
+    | Tnat, 0 => Some CO
+    | Tnat, 1 => Some CS
+
+    | Tbool, 0 => Some Cfalse
+    | Tbool, 1 => Some Ctrue
+
+    | Tlist_nat, 0 => Some Cnil
+    | Tlist_nat, 1 => Some Ccons
+
+    | _, _ => None
+    end.
+
+
